SepLogicTime/SepAuto.thy
@@ -2,17 +2,17 @@
    (by Lammich and Meis) in the AFP *)
 
 theory SepAuto
-  imports Auto2_HOL.SepLogic_Base "../Imperative_HOL"
-begin
+  imports Auto2_Imperative_HOL.SepLogic_Base "../Imperative_HOL"
+begin                         
 
-section {* Partial Heaps *}
+section \<open>Partial Heaps\<close>
 
 datatype pheap = pHeap (heapOf: heap) (addrOf: "addr set") (timeOf: nat)
-setup {* add_simple_datatype "pheap" *}
+setup \<open>add_simple_datatype "pheap"\<close>
 
 fun in_range :: "(heap \<times> addr set) \<Rightarrow> bool" where
   "in_range (h,as) \<longleftrightarrow> (\<forall>a\<in>as. a < lim h)"
-setup {* add_rewrite_rule @{thm in_range.simps} *}
+setup \<open>add_rewrite_rule @{thm in_range.simps}\<close>
 
 (* Two heaps agree on a set of addresses. *)
 definition relH :: "addr set \<Rightarrow> heap \<Rightarrow> heap \<Rightarrow> bool" where [rewrite]:
@@ -25,7 +25,7 @@ lemma relH_D [forward]:
 lemma relH_D2 [rewrite]:
   "relH as h h' \<Longrightarrow> a \<in> as \<Longrightarrow> refs h t a = refs h' t a"
   "relH as h h' \<Longrightarrow> a \<in> as \<Longrightarrow> arrays h t a = arrays h' t a" by auto2+
-setup {* del_prfstep_thm_eqforward @{thm relH_def} *}
+setup \<open>del_prfstep_thm_eqforward @{thm relH_def}\<close>
 
 lemma relH_dist_union [forward]:
   "relH (as \<union> as') h h' \<Longrightarrow> relH as h h' \<and> relH as' h h'" by auto2
@@ -46,13 +46,13 @@ lemma relH_set_array [resolve]:
   "relH {a. a < lim h \<and> a \<notin> {addr_of_array r}} h (Array.set r x h)"
   by (simp add: Array.set_def relH_def)
 
-section {* Assertions *}
+section \<open>Assertions\<close>
 
 datatype assn_raw = Assn (assn_fn: "pheap \<Rightarrow> bool")
 
 fun aseval :: "assn_raw \<Rightarrow> pheap \<Rightarrow> bool" where
   "aseval (Assn f) h = f h"
-setup {* add_rewrite_rule @{thm aseval.simps} *}
+setup \<open>add_rewrite_rule @{thm aseval.simps}\<close>
 
 definition proper :: "assn_raw \<Rightarrow> bool" where [rewrite]:
   "proper P = (
@@ -61,14 +61,14 @@ definition proper :: "assn_raw \<Rightarrow> bool" where [rewrite]:
 
 fun in_range_assn :: "pheap \<Rightarrow> bool" where
   "in_range_assn (pHeap h as n) \<longleftrightarrow> (\<forall>a\<in>as. a < lim h)"
-setup {* add_rewrite_rule @{thm in_range_assn.simps} *} 
+setup \<open>add_rewrite_rule @{thm in_range_assn.simps}\<close> 
 
 typedef assn = "Collect proper"
 @proof @have "Assn in_range_assn \<in> Collect proper" @qed
 
-setup {* add_rewrite_rule @{thm Rep_assn_inject} *}
-setup {* register_wellform_data ("Abs_assn P", ["proper P"]) *}
-setup {* add_prfstep_check_req ("Abs_assn P", "proper P") *}
+setup \<open>add_rewrite_rule @{thm Rep_assn_inject}\<close>
+setup \<open>register_wellform_data ("Abs_assn P", ["proper P"])\<close>
+setup \<open>add_prfstep_check_req ("Abs_assn P", "proper P")\<close>
 
 lemma Abs_assn_inverse' [rewrite]: "proper y \<Longrightarrow> Rep_assn (Abs_assn y) = y"
   by (simp add: Abs_assn_inverse)
@@ -90,7 +90,7 @@ instance .. end
 abbreviation one_assn :: assn ("emp") where "one_assn \<equiv> 1"
 
 lemma one_assn_rule [rewrite]: "h \<Turnstile> emp \<longleftrightarrow> timeOf h = 0 \<and> addrOf h = {}" by auto2
-setup {* del_prfstep_thm @{thm one_assn_def} *}
+setup \<open>del_prfstep_thm @{thm one_assn_def}\<close>
 
 section \<open>Definition of $\<close>
   
@@ -98,7 +98,7 @@ definition timeCredit_assn :: "nat \<Rightarrow> assn" ("$") where [rewrite]:
   "timeCredit_assn n = Abs_assn (Assn (\<lambda>h. timeOf h = n \<and> addrOf h = {}))"
     
 lemma timeCredit_assn_rule [rewrite]: "h \<Turnstile> $n \<longleftrightarrow> timeOf h = n \<and> addrOf h = {}" by auto2
-setup {* del_prfstep_thm @{thm timeCredit_assn_def} *}
+setup \<open>del_prfstep_thm @{thm timeCredit_assn_def}\<close>
 
 instantiation assn :: times begin
 definition times_assn where [rewrite]:
@@ -114,16 +114,16 @@ lemma mod_star_convE [backward]:
 lemma mod_star_convI [backward]:
   "as1 \<inter> as2 = {} \<Longrightarrow> pHeap h as1 n1 \<Turnstile> A \<Longrightarrow> pHeap h as2 n2 \<Turnstile> B \<Longrightarrow>
    pHeap h (as1 \<union> as2) (n1 + n2) \<Turnstile> A * B" by auto2
-setup {* del_prfstep_thm @{thm times_assn_def} *}
+setup \<open>del_prfstep_thm @{thm times_assn_def}\<close>
 
 lemma aseval_ext [backward]: "\<forall>h. aseval P h = aseval P' h \<Longrightarrow> P = P'"
   apply (cases P) apply (cases P') by auto
 
 lemma assn_ext: "\<forall>h as n. pHeap h as n \<Turnstile> P \<longleftrightarrow> pHeap h as n \<Turnstile> Q \<Longrightarrow> P = Q"
 @proof @have "Rep_assn P = Rep_assn Q" @qed
-setup {* add_backward_prfstep_cond @{thm assn_ext} [with_filt (order_filter "P" "Q")] *}
+setup \<open>add_backward_prfstep_cond @{thm assn_ext} [with_filt (order_filter "P" "Q")]\<close>
 
-setup {* del_prfstep_thm @{thm aseval_ext} *}
+setup \<open>del_prfstep_thm @{thm aseval_ext}\<close>
 
 lemma assn_one_left: "emp * P = (P::assn)"
 @proof
@@ -182,13 +182,13 @@ instantiation assn :: comm_monoid_mult begin
   apply (rule assn_times_assoc) apply (rule assn_times_comm) by (rule assn_one_left)
 end
 
-subsection {* Existential Quantification *}
+subsection \<open>Existential Quantification\<close>
 
 definition ex_assn :: "('a \<Rightarrow> assn) \<Rightarrow> assn" (binder "\<exists>\<^sub>A" 11) where [rewrite]:
   "(\<exists>\<^sub>Ax. P x) = Abs_assn (Assn (\<lambda>h. \<exists>x. h \<Turnstile> P x))"
 
 lemma mod_ex_dist [rewrite]: "(h \<Turnstile> (\<exists>\<^sub>Ax. P x)) \<longleftrightarrow> (\<exists>x. h \<Turnstile> P x)" by auto2
-setup {* del_prfstep_thm @{thm ex_assn_def} *}
+setup \<open>del_prfstep_thm @{thm ex_assn_def}\<close>
 
 lemma ex_distrib_star: "(\<exists>\<^sub>Ax. P x * Q) = (\<exists>\<^sub>Ax. P x) * Q"
 @proof
@@ -207,21 +207,21 @@ lemma ex_distrib_star: "(\<exists>\<^sub>Ax. P x * Q) = (\<exists>\<^sub>Ax. P x
   @end
 @qed
 
-subsection {* Disjunction *}
+subsection \<open>Disjunction\<close>
 
 definition or_assn :: "assn \<Rightarrow> assn \<Rightarrow> assn" (infixr "\<or>\<^sub>A" 61)  where [rewrite]:
   "A \<or>\<^sub>A B = Abs_assn (Assn (\<lambda>h. h\<Turnstile>A \<or> h\<Turnstile>B ) )"
 
 lemma or_assn_conv: "h \<Turnstile> A \<or>\<^sub>A B \<longleftrightarrow> (h \<Turnstile> A \<or> h \<Turnstile> B)" by auto2
 
-subsection {* Conjunction *}
+subsection \<open>Conjunction\<close>
 
 definition and_assn :: "assn \<Rightarrow> assn \<Rightarrow> assn" (infixr "\<and>\<^sub>A" 61)  where [rewrite]:
   "A \<and>\<^sub>A B = Abs_assn (Assn (\<lambda>h. h\<Turnstile>A \<and> h\<Turnstile>B ) )"
 
 lemma and_assn_conv: "h \<Turnstile> A \<and>\<^sub>A B \<longleftrightarrow> (h \<Turnstile> A \<and> h \<Turnstile> B)" by auto2
 
-subsection {* Pointers *}
+subsection \<open>Pointers\<close>
 
 definition sngr_assn :: "'a::heap ref \<Rightarrow> 'a \<Rightarrow> assn" (infix "\<mapsto>\<^sub>r" 82) where [rewrite]:
   "r \<mapsto>\<^sub>r x = Abs_assn (Assn (
@@ -230,7 +230,7 @@ definition sngr_assn :: "'a::heap ref \<Rightarrow> 'a \<Rightarrow> assn" (infi
 lemma sngr_assn_rule [rewrite]:
   "pHeap h as n \<Turnstile> r \<mapsto>\<^sub>r x \<longleftrightarrow>
       n = 0 \<and> Ref.get h r = x \<and> as = {addr_of_ref r} \<and> addr_of_ref r < lim h" by auto2
-setup {* del_prfstep_thm @{thm sngr_assn_def} *}
+setup \<open>del_prfstep_thm @{thm sngr_assn_def}\<close>
 
 definition snga_assn :: "'a::heap array \<Rightarrow> 'a list \<Rightarrow> assn" (infix "\<mapsto>\<^sub>a" 82) where [rewrite]:
   "r \<mapsto>\<^sub>a x = Abs_assn (Assn (
@@ -239,29 +239,29 @@ definition snga_assn :: "'a::heap array \<Rightarrow> 'a list \<Rightarrow> assn
 lemma snga_assn_rule [rewrite]:
   "pHeap h as n \<Turnstile> r \<mapsto>\<^sub>a x \<longleftrightarrow>
       (n = 0 \<and> Array.get h r = x \<and> as = {addr_of_array r} \<and> addr_of_array r < lim h)" by auto2
-setup {* del_prfstep_thm @{thm snga_assn_def} *}
+setup \<open>del_prfstep_thm @{thm snga_assn_def}\<close>
 
-subsection {* Pure Assertions *}
+subsection \<open>Pure Assertions\<close>
 
 definition pure_assn :: "bool \<Rightarrow> assn" ("\<up>") where [rewrite]:
   "\<up>b = Abs_assn (Assn (\<lambda>h. addrOf h = {} \<and> timeOf h = 0 \<and> b))"
 
 lemma pure_assn_rule [rewrite]: "h \<Turnstile> \<up>b \<longleftrightarrow> (addrOf h = {} \<and> timeOf h = 0 \<and> b)" by auto2
-setup {* del_prfstep_thm @{thm pure_assn_def} *}
+setup \<open>del_prfstep_thm @{thm pure_assn_def}\<close>
 
 definition top_assn :: assn ("true") where [rewrite]:
   "top_assn = Abs_assn (Assn in_range_assn)"
 
 lemma top_assn_rule [rewrite]: "pHeap h as n \<Turnstile> true \<longleftrightarrow> in_range (h, as)" by auto2
-setup {* del_prfstep_thm @{thm top_assn_def} *}
+setup \<open>del_prfstep_thm @{thm top_assn_def}\<close>
 
-setup {* del_prfstep_thm @{thm models_def} *}
+setup \<open>del_prfstep_thm @{thm models_def}\<close>
 
-subsection {* Properties of assertions *}
+subsection \<open>Properties of assertions\<close>
 
 abbreviation bot_assn :: assn ("false") where "bot_assn \<equiv> \<up>False"
 
-setup {* add_forward_prfstep @{thm mod_star_convE} *}
+setup \<open>add_forward_prfstep @{thm mod_star_convE}\<close>
 
 lemma mod_false' [resolve]: "\<not>(h \<Turnstile> false * R)" by auto2
 
@@ -293,11 +293,11 @@ lemma mod_timeCredit_dest [rewrite]:
 
 lemma pure_conj:  "\<up>(P \<and> Q) = \<up>P * \<up>Q" by auto2
 
-subsection {* Theorems for time credits *}
+subsection \<open>Theorems for time credits\<close>
 
 lemma time_credit_add [resolve]: "$(m + n) = $m * $n" by auto2
 
-subsection {* Entailment and its properties *}
+subsection \<open>Entailment and its properties\<close>
 
 definition entails :: "assn \<Rightarrow> assn \<Rightarrow> bool" (infix "\<Longrightarrow>\<^sub>A" 10) where [rewrite]:
   "(P \<Longrightarrow>\<^sub>A Q) \<longleftrightarrow> (\<forall>h. h \<Turnstile> P \<longrightarrow> h \<Turnstile> Q)"
@@ -322,11 +322,11 @@ lemma entails_ex: "\<not>((\<exists>\<^sub>Ax. P x) \<Longrightarrow>\<^sub>A Q)
 lemma entails_ex_post: "\<not>(P \<Longrightarrow>\<^sub>A (\<exists>\<^sub>Ax. Q x)) \<Longrightarrow> \<forall>x. \<not>(P \<Longrightarrow>\<^sub>A Q x)" by auto2
 lemma entails_pure_post: "\<not>(P \<Longrightarrow>\<^sub>A Q * \<up>b) \<Longrightarrow> P \<Longrightarrow>\<^sub>A Q \<Longrightarrow> \<not>b" by auto2
 
-setup {* del_prfstep_thm @{thm entails_def} *}
+setup \<open>del_prfstep_thm @{thm entails_def}\<close>
 
 definition time_credit_ge :: "nat \<Rightarrow> nat \<Rightarrow> bool" (infix "\<ge>\<^sub>t" 60) where
   "a \<ge>\<^sub>t b \<longleftrightarrow> a \<ge> b"
-setup {* add_backward_prfstep (equiv_backward_th @{thm time_credit_ge_def}) *}
+setup \<open>add_backward_prfstep (equiv_backward_th @{thm time_credit_ge_def})\<close>
 
 lemma gc_time': "a \<ge>\<^sub>t b \<Longrightarrow> R * $(a + p) \<Longrightarrow>\<^sub>A R * $(b + p) * true"
   by (smt assn_times_assoc assn_times_comm entails_frame gc_time time_credit_add time_credit_ge_def)
@@ -336,7 +336,7 @@ lemma gc_time'': "a \<ge>\<^sub>t b \<Longrightarrow> $(a + p) \<Longrightarrow>
 
 section \<open>Setup for timeFrame\<close>
     
-setup {* fold add_rewrite_rule @{thms timeFrame.simps} *}
+setup \<open>fold add_rewrite_rule @{thms timeFrame.simps}\<close>
 
 lemma timeFrame_reduceNone [forward]: "timeFrame n f = None \<Longrightarrow> f = None" by auto2
 
@@ -345,15 +345,15 @@ lemma timeFrame_reduceSome [forward]: "timeFrame n f = (Some (r,h,t)) \<Longrigh
 
 lemma zero_time: "$0 = emp" by auto2
 
-section {* Definition of the run predicate *}
+section \<open>Definition of the run predicate\<close>
 
 inductive run :: "'a Heap \<Rightarrow> heap option \<Rightarrow> heap option \<Rightarrow> 'a \<Rightarrow> nat \<Rightarrow> bool" where
   "run c None None r n"
 | "execute c h = None \<Longrightarrow> run c (Some h) None r n"
 | "execute c h = Some (r, h', n) \<Longrightarrow> run c (Some h) (Some h') r n"
-setup {* add_case_induct_rule @{thm run.cases} *}
-setup {* fold add_resolve_prfstep @{thms run.intros(1,2)} *}
-setup {* add_forward_prfstep @{thm run.intros(3)} *}
+setup \<open>add_case_induct_rule @{thm run.cases}\<close>
+setup \<open>fold add_resolve_prfstep @{thms run.intros(1,2)}\<close>
+setup \<open>add_forward_prfstep @{thm run.intros(3)}\<close>
 
 lemma run_complete [resolve]:
   "\<exists>\<sigma>' r n. run c \<sigma> \<sigma>' (r::'a) n"
@@ -367,15 +367,15 @@ lemma run_to_execute [forward]:
   "run c (Some h) \<sigma>' r n \<Longrightarrow> if \<sigma>' = None then execute c h = None else execute c h = Some (r, the \<sigma>', n)"
 @proof @case_induct "run c (Some h) \<sigma>' r n" @qed
 
-setup {* add_rewrite_rule @{thm execute_bind(1)} *}
+setup \<open>add_rewrite_rule @{thm execute_bind(1)}\<close>
 lemma runE [forward]:
   "run f (Some h) (Some h') r' t1 \<Longrightarrow> run (f \<bind> g) (Some h) \<sigma> r t \<Longrightarrow> run (g r') (Some h') \<sigma> r (t-t1)" by auto2
 
-setup {* add_rewrite_rule @{thm Array.get_alloc} *}
-setup {* add_rewrite_rule @{thm Ref.get_alloc} *}
-setup {* add_rewrite_rule_bidir @{thm Array.length_def} *}
+setup \<open>add_rewrite_rule @{thm Array.get_alloc}\<close>
+setup \<open>add_rewrite_rule @{thm Ref.get_alloc}\<close>
+setup \<open>add_rewrite_rule_bidir @{thm Array.length_def}\<close>
 
-section {* Definition of hoare triple, and the frame rule. *}
+section \<open>Definition of hoare triple, and the frame rule.\<close>
 
 definition new_addrs :: "heap \<Rightarrow> addr set \<Rightarrow> heap \<Rightarrow> addr set" where [rewrite]:
   "new_addrs h as h' = as \<union> {a. lim h \<le> a \<and> a < lim h'}"
@@ -389,7 +389,7 @@ lemma hoare_tripleD [forward]:
   "<P> c <Q> \<Longrightarrow> run c (Some h) \<sigma> r t \<Longrightarrow> \<forall>as n. pHeap h as n \<Turnstile> P \<longrightarrow>
     (\<sigma> \<noteq> None \<and> pHeap (the \<sigma>) (new_addrs h as (the \<sigma>)) (n-t) \<Turnstile> Q r \<and> n\<ge>t \<and> relH {a . a < lim h \<and> a \<notin> as} h (the \<sigma>) \<and>
      lim h \<le> lim (the \<sigma>))" by auto2
-setup {* del_prfstep_thm_eqforward @{thm hoare_triple_def} *}
+setup \<open>del_prfstep_thm_eqforward @{thm hoare_triple_def}\<close>
 
 abbreviation hoare_triple' :: "assn \<Rightarrow> 'r Heap \<Rightarrow> ('r \<Rightarrow> assn) \<Rightarrow> bool" ("<_> _ <_>\<^sub>t") where
   "<P> c <Q>\<^sub>t \<equiv> <P> c <\<lambda>r. Q r * true>"
@@ -409,7 +409,7 @@ lemma frame_rule [backward]:
 @qed
 
 (* This is the last use of the definition of separating conjunction. *)
-setup {* fold del_prfstep_thm [@{thm mod_star_convI}, @{thm mod_star_convE}] *}
+setup \<open>fold del_prfstep_thm [@{thm mod_star_convI}, @{thm mod_star_convE}]\<close>
 
 lemma bind_rule:
   "<P> f <Q> \<Longrightarrow> \<forall>x. <Q x> g x <R> \<Longrightarrow> <P> f \<bind> g <R>"
@@ -467,10 +467,10 @@ lemma gc_time_hoare': "a \<ge>\<^sub>t b \<Longrightarrow> \<not><R * $(a + p)> 
 
 lemma gc_time_hoare'': "a \<ge>\<^sub>t b \<Longrightarrow> \<not><$(a + p)> c <Q> \<Longrightarrow> \<not><$(b + p) * true> c <Q>"
 @proof @have "$(a+p) \<Longrightarrow>\<^sub>A $(b+p) * true" @qed
-setup {* del_prfstep_thm @{thm gc_time'} *}
-setup {* del_prfstep_thm @{thm gc_time''} *}
+setup \<open>del_prfstep_thm @{thm gc_time'}\<close>
+setup \<open>del_prfstep_thm @{thm gc_time''}\<close>
 
-setup {* fold del_prfstep_thm [@{thm entailsD}, @{thm entails_frame}, @{thm frame_rule}] *}
+setup \<open>fold del_prfstep_thm [@{thm entailsD}, @{thm entails_frame}, @{thm frame_rule}]\<close>
 
 (* Actual statement used: *)
 lemma post_rule':
@@ -479,10 +479,10 @@ lemma post_rule':
 lemma norm_pre_pure_iff: "<P * \<up>b> c <Q> \<longleftrightarrow> (b \<longrightarrow> <P> c <Q>)" by auto2
 lemma norm_pre_pure_iff2: "<\<up>b> c <Q> \<longleftrightarrow> (b \<longrightarrow> <emp> c <Q>)" by auto2
 
-section {* Hoare triples for atomic commands *}
+section \<open>Hoare triples for atomic commands\<close>
 
 (* First, those that do not modify the heap. *)
-setup {* add_rewrite_rule @{thm execute_assert(1)} *}
+setup \<open>add_rewrite_rule @{thm execute_assert(1)}\<close>
 lemma assert_rule:
   "<\<up>(R x) * $1> assert R x <\<lambda>r. \<up>(r = x)>" by auto2
 
@@ -490,34 +490,34 @@ lemma execute_return' [rewrite]: "execute (return x) h = Some (x, h, 1)" by (met
 lemma return_rule:
   "<$1> return x <\<lambda>r. \<up>(r = x)>" by auto2
 
-setup {* add_rewrite_rule @{thm execute_nth(1)} *}
+setup \<open>add_rewrite_rule @{thm execute_nth(1)}\<close>
 lemma nth_rule:
   "<a \<mapsto>\<^sub>a xs * $1 * \<up>(i < length xs)> Array.nth a i <\<lambda>r. a \<mapsto>\<^sub>a xs * \<up>(r = xs ! i)>" by auto2
 
-setup {* add_rewrite_rule @{thm execute_len} *}
+setup \<open>add_rewrite_rule @{thm execute_len}\<close>
 lemma length_rule:
   "<a \<mapsto>\<^sub>a xs * $1> Array.len a <\<lambda>r. a \<mapsto>\<^sub>a xs * \<up>(r = length xs)>" by auto2
 
-setup {* add_rewrite_rule @{thm execute_lookup} *}
+setup \<open>add_rewrite_rule @{thm execute_lookup}\<close>
 lemma lookup_rule:
   "<p \<mapsto>\<^sub>r x * $1> !p <\<lambda>r. p \<mapsto>\<^sub>r x * \<up>(r = x)>" by auto2
     
-setup {* add_rewrite_rule @{thm execute_freeze} *}
+setup \<open>add_rewrite_rule @{thm execute_freeze}\<close>
 lemma freeze_rule:
   "<a \<mapsto>\<^sub>a xs * $(1 + length xs)> Array.freeze a <\<lambda>r. a \<mapsto>\<^sub>a xs * \<up>(r = xs)>" by auto2
 
 (* Next, the update rules. *)
-setup {* add_rewrite_rule @{thm Ref.lim_set} *}
+setup \<open>add_rewrite_rule @{thm Ref.lim_set}\<close>
 lemma Array_lim_set [rewrite]: "lim (Array.set p xs h) = lim h" by (simp add: Array.set_def)
 
-setup {* fold add_rewrite_rule [@{thm Ref.get_set_eq}, @{thm Array.get_set_eq}] *}
-setup {* add_rewrite_rule @{thm Array.update_def} *}
+setup \<open>fold add_rewrite_rule [@{thm Ref.get_set_eq}, @{thm Array.get_set_eq}]\<close>
+setup \<open>add_rewrite_rule @{thm Array.update_def}\<close>
 
-setup {* add_rewrite_rule @{thm execute_upd(1)} *}
+setup \<open>add_rewrite_rule @{thm execute_upd(1)}\<close>
 lemma upd_rule:
   "<a \<mapsto>\<^sub>a xs * $1 * \<up>(i < length xs)> Array.upd i x a <\<lambda>r. a \<mapsto>\<^sub>a list_update xs i x * \<up>(r = a)>" by auto2
 
-setup {* add_rewrite_rule @{thm execute_update} *}
+setup \<open>add_rewrite_rule @{thm execute_update}\<close>
 lemma update_rule:
   "<p \<mapsto>\<^sub>r y * $1> p := x <\<lambda>r. p \<mapsto>\<^sub>r x>" by auto2
 
@@ -528,8 +528,8 @@ lemma Array_alloc_def' [rewrite]:
   "Array.alloc xs h = (let l = lim h; r = Array l in (r, (Array.set r xs (h\<lparr>lim := l + 1\<rparr>))))"
   by (simp add: Array.alloc_def)
 
-setup {* fold add_rewrite_rule [
-  @{thm addr_of_array.simps}, @{thm addr_of_ref.simps}, @{thm Ref.alloc_def}] *}
+setup \<open>fold add_rewrite_rule [
+  @{thm addr_of_array.simps}, @{thm addr_of_ref.simps}, @{thm Ref.alloc_def}]\<close>
 
 lemma refs_on_Array_set [rewrite]: "refs (Array.set p xs h) t i = refs h t i"
   by (simp add: Array.set_def)
@@ -551,30 +551,30 @@ lemma refs_on_Ref_alloc [rewrite]: "i < lim h \<Longrightarrow> refs (snd (Ref.a
   by (smt Ref.alloc_def Ref.set_def addr_of_ref.simps fun_upd_apply less_or_eq_imp_le
           linorder_not_less select_convs(2) simps(6) snd_conv surjective update_convs(3))
 
-setup {* add_rewrite_rule @{thm execute_new} *}
+setup \<open>add_rewrite_rule @{thm execute_new}\<close>
 lemma new_rule:
   "<$(n+1)> Array.new n x <\<lambda>r. r \<mapsto>\<^sub>a replicate n x>" by auto2
 
 
-setup {* add_rewrite_rule @{thm execute_make} *}
+setup \<open>add_rewrite_rule @{thm execute_make}\<close>
 lemma make_rule:
   "<$(n+1)> Array.make n f <\<lambda>r. r \<mapsto>\<^sub>a map f [0 ..< n]>" by auto2
 
-setup {* add_rewrite_rule @{thm execute_of_list} *}
+setup \<open>add_rewrite_rule @{thm execute_of_list}\<close>
 lemma of_list_rule:
   "<$ (1+length xs)> Array.of_list xs <\<lambda>r. r \<mapsto>\<^sub>a xs>" by auto2
 
-setup {* add_rewrite_rule @{thm execute_ref} *}
+setup \<open>add_rewrite_rule @{thm execute_ref}\<close>
 lemma ref_rule:
   "<$1> ref x <\<lambda>r. r \<mapsto>\<^sub>r x>" by auto2
 
-setup {* fold del_prfstep_thm [
+setup \<open>fold del_prfstep_thm [
   @{thm sngr_assn_rule}, @{thm snga_assn_rule}, @{thm pure_assn_rule}, @{thm top_assn_rule},
   @{thm mod_pure_star_dist}, @{thm one_assn_rule}, @{thm hoare_triple_def}, @{thm mod_ex_dist},
-  @{thm mod_timeCredit_dest}, @{thm timeCredit_assn_rule}] *}
-setup {* del_simple_datatype "pheap" *}
+  @{thm mod_timeCredit_dest}, @{thm timeCredit_assn_rule}]\<close>
+setup \<open>del_simple_datatype "pheap"\<close>
 
-subsection {* Definition of procedures *}
+subsection \<open>Definition of procedures\<close>
 
 (* ASCII abbreviations for ML files. *)
 abbreviation (input) ex_assn_ascii :: "('a \<Rightarrow> assn) \<Rightarrow> assn" (binder "EXA" 11)
@@ -589,7 +589,7 @@ ML_file "sep_time_util.ML"
 ML_file "sep_util.ML"
 ML_file "sep_time_steps.ML"
 
-ML {*
+ML \<open>
 structure AssnMatcher = AssnMatcher(SepUtil)
 structure SepLogic = SepLogic(SepUtil)
 structure SepTimeSteps = SepTimeSteps(SepUtil)
@@ -598,23 +598,23 @@ val add_entail_matcher = AssnMatcher.add_entail_matcher
 val add_forward_ent_prfstep = SepLogic.add_forward_ent_prfstep
 val add_rewrite_ent_rule = SepLogic.add_rewrite_ent_rule
 val add_hoare_triple_prfstep = SepLogic.add_hoare_triple_prfstep
-*}
+\<close>
 
 (* Make sure to add time proofsteps first (execute time_credit_ge first) *)
-setup {* SepTimeSteps.add_time_proofsteps *}
-setup {* AssnMatcher.add_assn_matcher_proofsteps *}
-setup {* SepLogic.add_sep_logic_proofsteps *}
+setup \<open>SepTimeSteps.add_time_proofsteps\<close>
+setup \<open>AssnMatcher.add_assn_matcher_proofsteps\<close>
+setup \<open>SepLogic.add_sep_logic_proofsteps\<close>
 
 ML_file "sep_time_test.ML"
 
-attribute_setup forward_ent = {* setup_attrib add_forward_ent_prfstep *}
-attribute_setup rewrite_ent = {* setup_attrib add_rewrite_ent_rule *}
-attribute_setup hoare_triple = {* setup_attrib add_hoare_triple_prfstep *}
+attribute_setup forward_ent = \<open>setup_attrib add_forward_ent_prfstep\<close>
+attribute_setup rewrite_ent = \<open>setup_attrib add_rewrite_ent_rule\<close>
+attribute_setup hoare_triple = \<open>setup_attrib add_hoare_triple_prfstep\<close>
 
-setup {* fold add_hoare_triple_prfstep [
+setup \<open>fold add_hoare_triple_prfstep [
   @{thm assert_rule}, @{thm update_rule}, @{thm nth_rule}, @{thm upd_rule},
   @{thm return_rule}, @{thm ref_rule}, @{thm lookup_rule}, @{thm new_rule},
-  @{thm make_rule}, @{thm of_list_rule}, @{thm length_rule}, @{thm freeze_rule}] *}
+  @{thm make_rule}, @{thm of_list_rule}, @{thm length_rule}, @{thm freeze_rule}]\<close>
 
 (* Some simple tests *)
 
